src/coq/Semantics/Memory/Sizeof.v
@@ -3,10 +3,25 @@ From Coq Require Import
          List.
 
 From Vellvm Require Import
-     DynamicTypes.
+  DynamicTypes
+  Utils.ListUtil.
 
-Definition pad_to (pad_amount : N) (sz : N) :=
-  (sz + ((pad_amount - (sz mod pad_amount)) mod pad_amount))%N.
+Definition pad_amount (alignment : N) (offset : N) :=
+  ((alignment - (offset mod alignment)) mod alignment)%N.
+
+Definition pad_to (alignment : N) (sz : N) :=
+  (sz + pad_amount alignment sz)%N.
+
+Record alignment :=
+  { abi_alignment : N  (** Required alignment in bytes *)
+  ; preferred_alignment : N  (** Preferred alignment in bytes *)
+  }.
+
+Definition pad_to_align (align : alignment) (sz : N) :=
+  pad_to (preferred_alignment align) sz.
+
+Definition pad_to_align_bitwise (align : alignment) (sz : N) :=
+  pad_to ((preferred_alignment align) * 8) sz.
 
 Module Type Sizeof.
   (** ** Size of a dynamic type in bits *)
@@ -21,20 +36,27 @@ Module Type Sizeof.
     forall dt,
       (0 <= sizeof_dtyp dt)%N.
 
-  Parameter padding : N.
+  (** Alignment of a dtyp *)
+  Parameter dtyp_alignment : dtyp -> alignment.
 
-  (* Should take padding into account *)
+  Definition max_preferred_dtyp_alignment (dts : list dtyp) : N :=
+    match maximumByOpt (fun dt1 dt2 => preferred_alignment (dtyp_alignment dt1) <? preferred_alignment (dtyp_alignment dt1))%N dts with
+    | Some dt =>
+        preferred_alignment (dtyp_alignment dt)
+    | None => 1
+    end.
+
   Parameter sizeof_dtyp_Struct :
     forall dts,
-      sizeof_dtyp (DTYPE_Struct dts) = List.fold_left (fun acc dt => N.add acc (pad_to padding (sizeof_dtyp dt))) dts 0%N.
-
+      sizeof_dtyp (DTYPE_Struct dts) = pad_to (max_preferred_dtyp_alignment dts) (List.fold_left (fun acc dt => N.add (pad_to_align (dtyp_alignment dt) acc) (sizeof_dtyp dt)) dts 0%N).
+    
   Parameter sizeof_dtyp_Packed_struct :
     forall dts,
       sizeof_dtyp (DTYPE_Packed_struct dts) = List.fold_left (fun acc dt => N.add acc (sizeof_dtyp dt)) dts 0%N.
 
   Parameter sizeof_dtyp_array :
     forall sz t,
-      sizeof_dtyp (DTYPE_Array sz t) = (sz * (pad_to padding (sizeof_dtyp t)))%N.
+      sizeof_dtyp (DTYPE_Array sz t) = (sz * sizeof_dtyp t)%N.
 
   Parameter sizeof_dtyp_vector :
     forall sz t,
